src/ExpSyntax.v
@@ -11,31 +11,42 @@ Import ListNotations.
 
 (** The syntax of expressions: *)
 Inductive Exp : Set :=
-| ELit    (l : Lit)
-| EPid    (p : PID)
-(** Variables and function identifiers are just indices.
-    TODO: In the future, function identifiers should include the arity too!
-*)
-| EVar    (n : nat)
-(** Instead of multiple fun constructs (recursive and non-recursive), 
-    we use only recursive funs, which use the 0 DB-index as the recursive fun-exp *)
-| VFun    (vl : nat) (e : Exp)
+| EExp (e : NonVal)
+| VVal (v : Val)
+
+with NonVal : Set :=
 | EApp    (exp : Exp)     (l : list Exp)
 | ELet    (e1 e2 : Exp)
 (** Eliminator *)
 | ECase (e : Exp) (p : Pat) (e1 e2 : Exp)
 (** Lists *)
 | ECons (e1 e2 : Exp)
-| ENil
-(** Recursive data structures which are values: *)
-| VCons (e1 e2 : Exp)
-(** Concurrency *)
 | EReceive (l : list (Pat * Exp))
 | EBIF (e : Exp) (l : list Exp)
 (** We note, that both sequential and concurrent built-in functions
     are represented by EBIF, just like in Core Erlang itself.
 *)
+
+with Val : Set :=
+| VLit    (l : Lit)
+| VPid    (p : PID)
+| VVar    (n : nat)
+(** Instead of multiple fun constructs (recursive and non-recursive), 
+    we use only recursive funs, which use the 0 DB-index as the recursive fun-exp *)
+| VFun    (vl : nat) (e : Exp)
+| VNil
+(** Recursive data structures which are values: *)
+| VCons (e1 e2 : Val)
+(** Concurrency *)
 .
+
+Declare Scope sub_scope.
+Delimit Scope sub_scope with sub.
+
+Coercion EExp : NonVal >-> Exp.
+Coercion VVal : Val >-> Exp.
+Notation "˝ v" := (VVal v) (at level 11) : sub_scope.
+Notation "° n" := (EExp n) (at level 11) : sub_scope.
 
 Section correct_exp_ind.
 (** Coq cannot automatically generate correct induction principle
@@ -43,23 +54,29 @@ Section correct_exp_ind.
     and list). Thus we define it by hand:
 *)
   Variables
-    (P : Exp -> Prop)(Q : list Exp -> Prop)(W : list (Pat * Exp) -> Prop).
+    (P : Exp -> Prop)
+    (PV : Val -> Prop)
+    (PN : NonVal -> Prop)
+    (Q : list Exp -> Prop)
+    (W : list (Pat * Exp) -> Prop).
 
   Hypotheses
-   (H0 : forall (l : Lit), P (ELit l))
-   (H00 : forall (l : PID), P (EPid l))
-   (H1 : forall (n : nat), P (EVar n))
-   (H3 : forall (vl : nat) (e : Exp), P e -> P (VFun vl e))
+   (HE1 : forall v : Val, PV v -> P (VVal v))
+   (HE2 : forall v : NonVal, PN v -> P (EExp v))
+   (H0 : forall (l : Lit), PV (VLit l))
+   (H00 : forall (l : PID), PV (VPid l))
+   (H1 : forall (n : nat), PV (VVar n))
+   (H3 : forall (vl : nat) (e : Exp), P e -> PV (VFun vl e))
    (H5 : forall (e : Exp), P e -> forall (el : list Exp), Q el 
-       -> P (EApp e el))
+       -> PN (EApp e el))
    (H6 : forall (e1 : Exp), P e1 -> forall e2 : Exp, P e2 
-       -> P (ELet e1 e2))
-   (H9 : forall (e1 : Exp), P e1 ->  forall e2, P e2 -> forall e3, P e3 -> forall p, P (ECase e1 p e2 e3))
-   (H10 : forall e1, P e1 -> forall e2, P e2 -> P (ECons e1 e2))
-   (H11 : P ENil)
-   (H12 : forall e1, P e1 -> forall e2, P e2 -> P (VCons e1 e2))
-   (H13 : forall e1, P e1 -> forall l, Q l -> P (EBIF e1 l))
-   (H14 : forall l, W l -> P (EReceive l))
+       -> PN (ELet e1 e2))
+   (H9 : forall (e1 : Exp), P e1 ->  forall e2, P e2 -> forall e3, P e3 -> forall p, PN (ECase e1 p e2 e3))
+   (H10 : forall e1, P e1 -> forall e2, P e2 -> PN (ECons e1 e2))
+   (H11 : PV VNil)
+   (H12 : forall e1, PV e1 -> forall e2, PV e2 -> PV (VCons e1 e2))
+   (H13 : forall e1, P e1 -> forall l, Q l -> PN (EBIF e1 l))
+   (H14 : forall l, W l -> PN (EReceive l))
    (H1' : Q [])
    (H'  : forall e, P e -> forall l, Q l -> Q (e :: l))
    (J : W [])
@@ -67,10 +84,11 @@ Section correct_exp_ind.
 
   Fixpoint Exp_ind2 (e : Exp) : P e :=
   match e as x return P x with
-  | ELit l => H0 l
-  | EPid l => H00 l
-  | EVar n => H1 n
-  | VFun vl e => H3 vl e (Exp_ind2 e)
+  | VVal v => HE1 v (Val_ind2 v)
+  | EExp e => HE2 e (NonVal_ind2 e)
+  end
+  with NonVal_ind2 (e : NonVal) : PN e :=
+  match e as x return PN x with
   | EApp e el => H5 e (Exp_ind2 e) el ((fix l_ind (l':list Exp) : Q l' :=
                                          match l' as x return Q x with
                                          | [] => H1'
@@ -79,8 +97,6 @@ Section correct_exp_ind.
   | ELet e1 e2 => H6 e1 (Exp_ind2 e1) e2 (Exp_ind2 e2)
   | ECase e p e1 e2 => H9 e (Exp_ind2 e) e1 (Exp_ind2 e1) e2 (Exp_ind2 e2) p
   | ECons e1 e2 => H10 e1 (Exp_ind2 e1) e2 (Exp_ind2 e2)
-  | ENil => H11
-  | VCons e1 e2 => H12 e1 (Exp_ind2 e1) e2 (Exp_ind2 e2)
   | EBIF e l => H13 e (Exp_ind2 e) l ((fix l_ind (l':list Exp) : Q l' :=
                                          match l' as x return Q x with
                                          | [] => H1'
@@ -91,50 +107,61 @@ Section correct_exp_ind.
                                          | [] => J
                                          | (p, v)::xs => J0 v (Exp_ind2 v) xs (l_ind xs) p
                                          end) l)
+  end
+  with Val_ind2 (e : Val) : PV e :=
+  match e as x return PV x with
+  | VLit l => H0 l
+  | VPid l => H00 l
+  | VVar n => H1 n
+  | VFun vl e => H3 vl e (Exp_ind2 e)
+  | VNil => H11
+  | VCons e1 e2 => H12 e1 (Val_ind2 e1) e2 (Val_ind2 e2)
   end.
 
 End correct_exp_ind.
 
-Fixpoint Exp_eq_dec (e e' : Exp) : {e = e'} + {e <> e'}.
-Proof. repeat decide equality. Qed.
+Fixpoint Exp_eq_dec (e e' : Exp) : {e = e'} + {e <> e'}
+with NonVal_eq_dec (e e' : NonVal) : {e = e'} + {e <> e'}
+with Val_eq_dec (e e' : Val) : {e = e'} + {e <> e'}.
+Proof. all: repeat decide equality. Qed.
 
 (** Examples *)
-
+Open Scope sub_scope.
 (** Incrementing expression *)
-Definition inc (n : Z) := ELet (ELit n) (EBIF (ELit "+"%string) [EVar 0; ELit 1%Z]).
+Definition inc (n : Z) := ELet (VLit n) (EBIF (VLit "+"%string) [˝VVar 0; ˝VLit 1%Z]).
 (** Summation from 0 to the given positive number *)
-Definition sum (n : Z) := ELet (VFun 1 (ECase (EVar 1) (PLit 0%Z) (EVar 1) (
-                                            (EBIF (ELit "+"%string) [EVar 1;
-                                            EApp (EVar 0) [EBIF (ELit "+"%string) [EVar 1; ELit ((-1)%Z)]]]))))
-                        (EApp (EVar 0) [ELit n]).
+Definition sum (n : Z) := ELet (VFun 1 (ECase (VVar 1) (PLit 0%Z) (VVar 1) (
+                                            (EBIF (VLit "+"%string) [˝VVar 1;
+                                            °EApp (VVar 0) [°EBIF (VLit "+"%string) [˝VVar 1; ˝VLit ((-1)%Z)]]]))))
+                        (EApp (˝VVar 0) [˝VLit n]).
 (** Application of a 0-parameter function inside `let`. *)
-Definition simplefun (n : Z) := ELet XVar (EFun [] (ELit n)) (EApp (EVar 0) []).
+Definition simplefun (n : Z) := ELet (VFun 0 (VLit n)) (EApp (VVar 0) []).
 (** Application of a two-parameter function, which sums these. *)
-Definition simplefun2 (n m : Z) := EApp (EFun [XVar; YVar] (EBIF (ELit "+"%string) [EVar 1; EVar 2])) [ELit n; ELit m].
+Definition simplefun2 (n m : Z) := EApp (VFun 2 (EBIF (VLit "+"%string) [˝VVar 1; ˝VVar 2])) [˝VLit n; ˝VLit m].
 
 (** Map function expressed with `letrec`. It transforms the list with
     the given function value. *)
 Definition obj_map f e : Exp :=
-  ELetRec MAP [FVar;XVar]
-    (ECase (EVar 2)
-      (PCons PVar PVar) (ECons (EApp (EVar 3) [EVar 0])
-                               (EApp (EFunId 2) [EVar 3; EVar 1]))
-                        ENil
-    )
-    (EApp (EFunId 0) [f;e]).
+  ELet (VFun 2
+    (ECase (VVar 2)
+      (PCons PVar PVar) (ECons (EApp (VVar 3) [˝VVar 0])
+                               (EApp (VVar 2) [˝VVar 3; ˝VVar 1]))
+                        VNil
+    ))
+    (EApp (VVar 0) [f;e]).
 
 (** Foldr function expressed with `letrec`. It aggregates a list. *)
 Definition obj_foldr f e d : Exp :=
-  ELetRec FOLDR [FVar;DVar;XVar]
-    (ECase (EVar 3)
-      (PCons PVar PVar) (EApp (EVar 3) [EVar 0; EApp (EFunId 2) [EVar 3; EVar 4; EVar 1]])
-                        (EVar 2)
-    )
-    (EApp (EFunId 0) [f;d;e]).
+  ELet (VFun 3
+    (ECase (VVar 3)
+      (PCons PVar PVar) (EApp (VVar 3) [˝VVar 0; °EApp (VVar 2) [˝VVar 3; ˝VVar 4; ˝VVar 1]])
+                        (VVar 2)
+    ))
+    (EApp (VVar 0) [f;d;e]).
 
 (** Names, equalities *)
 
-(* The equality of function signatures *)
+(* (* The equality of function signatures *)
 Definition funid_eqb (v1 v2 : FunctionIdentifier) : bool :=
 match v1, v2 with
 | (fid1, num1), (fid2, num2) => String.eqb fid1 fid2 && Nat.eqb num1 num2
@@ -238,7 +265,7 @@ Proof.
   * destruct f. simpl. rewrite eqb_refl, Nat.eqb_refl. simpl. reflexivity.
 Qed.
 
-Global Hint Resolve var_funid_eqb_refl : core.
+Global Hint Resolve var_funid_eqb_refl : core. *)
 
 Section in_list.
 (** Bool-based In for Coq *)
@@ -278,9 +305,7 @@ Proof.
       + inversion H.
       + apply eqb_false in Heqb. simpl. intro. inversion H0. symmetry in H1. contradiction.
         eapply IHl; eauto.
-    - simpl. break_match_goal.
-      apply eqb_true in Heqb. subst. exfalso. apply H. intuition.
-      apply eqb_false in Heqb. eapply IHl. apply not_in_cons in H. destruct H. auto.
+    - simpl. break_match_goal. set_solver. set_solver.
 Qed.
 
 End in_list.
@@ -296,15 +321,15 @@ Fixpoint match_pattern (p : Pat) (e : Exp) : option (list Exp) :=
 match p with
 | PVar => Some [e]
 | PPid x => match e with
-            | EPid p => if Nat.eqb p x then Some [] else None
+            | VPid p => if Nat.eqb p x then Some [] else None
             | _      => None
             end
 | PNil => match e with
-          | ENil => Some []
+          | VNil => Some []
           | _    => None
           end
 | PLit l0 => match e with
-             | ELit l => if lit_eqb l l0 then Some [] else None
+             | VLit l => if lit_eqb l l0 then Some [] else None
              | _      => None
              end
 | PCons p1 p2 => 
@@ -331,11 +356,12 @@ Lemma match_pattern_length : forall p v l,
   match_pattern p v = Some l -> pat_vars p = length l.
 Proof.
   induction p; intros.
-  * simpl in *. destruct v; inversion H. break_match_hyp; now inversion H.
-  * simpl in *. destruct v; inversion H. break_match_hyp; now inversion H.
+  * simpl in *. destruct v; inversion H. destruct v; try break_match_hyp; by inversion H.
+  * simpl in *. destruct v; inversion H. destruct v; try break_match_hyp; by inversion H.
   * simpl in *. destruct v; inversion H; subst; auto.
-  * simpl in *. destruct v; inversion H. subst. auto.
-  * simpl. simpl in H. destruct v; try congruence.
+  * simpl in *. destruct v; inversion H. destruct v; subst; try congruence.
+    by inversion H.
+  * simpl. simpl in H. destruct v; try congruence. destruct v; try congruence.
     break_match_hyp; try congruence. break_match_hyp; try congruence. inversion H.
     subst. erewrite length_app, IHp1, IHp2. reflexivity. all: eauto.
 Qed.
